Add functions

src/defs/dynamics.lean
@@ -1,9 +1,11 @@
 import defs.syntax
+import defs.subst
 
 inductive val: exp -> Prop
 | int (n: ℤ): val (exp.int n)
 | true: val exp.true
 | false: val exp.false
+| fn (x: var) (τ: typ) (e: exp): val (exp.fn x τ e)
 
 inductive steps: exp -> exp -> Prop
 | if_e1
@@ -16,3 +18,17 @@ inductive steps: exp -> exp -> Prop
 | if_false
     (e2 e3: exp):
     steps (exp.if_ exp.false e2 e3) e3
+| app_e1
+    (e1 e1' e2: exp):
+    steps e1 e1' ->
+    steps (exp.app e1 e2) (exp.app e1' e2)
+| app_e2
+    (e1 e2 e2': exp):
+    val e1 ->
+    steps e2 e2' ->
+    steps (exp.app e1 e2) (exp.app e1 e2')
+| app_done
+    (x: var) (τ: typ) (e e2 e': exp):
+    val e2 ->
+    subst (list.cons (prod.mk x e2) list.nil) e e' ->
+    steps (exp.app (exp.fn x τ e) e2) e'
