src/defs/statics.lean
@@ -11,3 +11,16 @@ inductive has_typ: cx typ -> exp -> typ -> Prop
     has_typ Γ e2 τ ->
     has_typ Γ e3 τ ->
     has_typ Γ (exp.if_ e1 e2 e3) τ
+| var
+    (Γ: cx typ) (x: var) (τ: typ):
+    lookup Γ x τ ->
+    has_typ Γ (exp.var x) τ
+| fn
+    (Γ: cx typ) (x: var) (τ1 τ2: typ) (e: exp):
+    has_typ (list.cons (prod.mk x τ1) Γ) e τ2 ->
+    has_typ Γ (exp.fn x τ1 e) (typ.arrow τ1 τ2)
+| app
+    (Γ: cx typ) (e1 e2: exp) (τ1 τ2: typ):
+    has_typ Γ e1 (typ.arrow τ1 τ2) ->
+    has_typ Γ e2 τ1 ->
+    has_typ Γ (exp.app e1 e2) τ2
