src/defs/syntax.lean
@@ -3,9 +3,13 @@ import defs.var
 inductive typ: Type
 | int: typ
 | bool: typ
+| arrow: typ -> typ -> typ
 
 inductive exp: Type
 | int: ℤ -> exp
 | true: exp
 | false: exp
 | if_: exp -> exp -> exp -> exp
+| var: var -> exp
+| fn: var -> typ -> exp -> exp
+| app: exp -> exp -> exp
