src/defs/subst.lean
@@ -1,4 +1,5 @@
 import defs.syntax
+import defs.fv
 
 inductive subst: cx exp -> exp -> exp -> Prop
 | int (Δ: cx exp) (n: ℤ): subst Δ (exp.int n) (exp.int n)
@@ -11,3 +12,22 @@ inductive subst: cx exp -> exp -> exp -> Prop
     subst Δ e2 e2' ->
     subst Δ e3 e3' ->
     subst Δ (exp.if_ e1 e2 e3) (exp.if_ e1' e2' e3')
+| var_same
+    (Δ: cx exp) (x: var) (e': exp):
+    lookup Δ x e' ->
+    subst Δ (exp.var x) e'
+| var_diff
+    (Δ: cx exp) (x: var):
+    (∀ p ∈ Δ, prod.fst p ≠ x) ->
+    subst Δ (exp.var x) (exp.var x)
+| fn
+    (Δ: cx exp) (x x': var) (τ: typ) (e e': exp):
+    (∀ a ∈ list.cons e (list.map prod.snd Δ), x' ∉ fv a) ->
+    subst (list.cons (prod.mk x (exp.var x')) Δ) e e' ->
+    subst Δ (exp.fn x τ e) (exp.fn x' τ e')
+| app
+    (Δ: cx exp)
+    (e1 e1' e2 e2': exp):
+    subst Δ e1 e1' ->
+    subst Δ e2 e2' ->
+    subst Δ (exp.app e1 e2) (exp.app e1' e2')
