src/lemmas/canonical_forms.lean
@@ -12,4 +12,19 @@ begin
   right,
   refl,
   cases value,
+  cases value,
+  cases value,
+end
+
+theorem arrow_canonical_forms
+  {Γ: cx typ} {e: exp} {τ1 τ2: typ} (value: val e)
+  (et: has_typ Γ e (typ.arrow τ1 τ2))
+  : ∃ (x: var) (e': exp), e = exp.fn x τ1 e' :=
+begin
+  cases et,
+  cases value,
+  cases value,
+  existsi [et_x, et_e],
+  refl,
+  cases value,
 end
